src/Framework/ReflComp.v
@@ -428,10 +428,10 @@ Section Linking.
      1. e1 and e2 can contain multiple holes
      2. f can be either free or not in either e1 or e2 as long as e1 is compiled by the pipeline.
      3. x can be either free or not in e2 as long as e2 is compiled by the pipeline.
-     4. w needs to be exposed *)
-  Definition link f w x e1 e2 : exp :=
-    Efun f w [] e1
-      (Eletapp x f w [] e2).
+     4. w needs to be exposed
+
+     Print link.
+   *)
 
   (* Note the following lemma is not applicable as [trans_correct] is not the top-level relation.
    * Thus, we need to show the compat lemmas for fun and letapp with [related_top] *)
